Fix issue with free vars and types_wf, extract and test
binding equal to free vars minus bound vars
fixed this condition, proofs
remove extra uneeded removal in sub definition

extract/TheoryImports.ml
@@ -16,9 +16,9 @@ open State
 open Base
 open Fin_maps
 open Hashcons
-open Pmap
+open Pmap0
 open Strings0
-open Zmap
+open Zmap0
 
 open Format
 open Ident
